Prove a correctness result for a cmlPtreeConversion function
The result states that the conversion function that takes a parse tree
to an AST type value has a right-inverse (a printing function if you
will), as long as the AST value is "user-expressible". Some AST values
in this type can't be expressed in the parse trees. For example, the
built-in type constructors TC_int etc are outside of the range of the
conversion, as is the "for internal use" Tvar_db.

Moreover, show that the ptree_Type function always hits
user-expressible types.

In retrspect, we should have proved analogous theorems for all of the
conversion functions as part of our correctness argument for the
parser.

semantics/proofs/cmlPtreeConversionPropsScript.sml
@@ -10,6 +10,173 @@ val _ = set_grammar_ancestry ["cmlPtreeConversion", "gramProps"]
 val _ = export_rewrites ["option.OPTION_IGNORE_BIND_def"]
 (* " *)
 
+(* a function for mapping types back to ASTs, used to check that the
+   conversion functions are doing something reasonable *)
+
+(* first, capture those types that we expect to be in the range of the
+   conversion *)
+val user_expressible_tyname_def = Define‘
+  (user_expressible_tyname (Short s) ⇔ T) ∧
+  (user_expressible_tyname (Long m (Short s)) ⇔ T) ∧
+  (user_expressible_tyname _ ⇔ F)
+’;
+val _ = augment_srw_ss [rewrites [user_expressible_tyname_def]]
+
+val _ = temp_overload_on ("ND", “λn. Nd (mkNT n, ARB)”)
+val _ = temp_overload_on ("LF", “λt. Lf (TOK t, ARB)”)
+val tyname_to_AST_def = Define‘
+  tyname_to_AST (Short n) = ND nTyOp [ND nUQTyOp [LF (AlphaT n)]] ∧
+  tyname_to_AST (Long md (Short n)) = ND nTyOp [LF (LongidT md n)] ∧
+  tyname_to_AST _ = ARB
+’;
+
+val tyname_inverted = Q.store_thm(
+  "tyname_inverted",
+  ‘∀id. user_expressible_tyname id ⇒
+        ptree_Tyop (tyname_to_AST id) = SOME id’,
+  Cases >>
+  simp[ptree_Tyop_def, tyname_to_AST_def, ptree_UQTyop_def] >>
+  rename [‘Long m j’] >> Cases_on ‘j’ >>
+  simp[ptree_Tyop_def, tyname_to_AST_def, ptree_UQTyop_def]);
+
+val user_expressible_type_def = tDefine "user_expressible_type" ‘
+  (user_expressible_type (Tvar _) ⇔ T) ∧
+  (user_expressible_type (Tvar_db _) ⇔ F) ∧
+  (user_expressible_type (Tapp tys tycon) ⇔
+     EVERY user_expressible_type tys ∧
+     ((∃id. tycon = TC_name id ∧ user_expressible_tyname id) ∨
+      (∃d r. tys = [d;r] ∧ tycon = TC_fn) ∨
+      (tycon = TC_tup ∧ 2 ≤ LENGTH tys)))
+’ (WF_REL_TAC ‘measure ast$t_size’ >> simp[] >> rpt gen_tac >>
+   Induct_on ‘tys’ >>
+   dsimp[astTheory.t_size_def] >> rpt strip_tac >> res_tac  >> simp[]);
+val _ = augment_srw_ss [rewrites [
+           SIMP_RULE (srw_ss() ++ ETA_ss) [] user_expressible_type_def]]
+
+val type_to_AST_def = tDefine "type_to_AST" ‘
+  type_to_AST (Tvar s) : (token,MMLnonT,unit) parsetree =
+    ND nType [ND nPType [ND nDType [ND nTbase [LF (TyvarT s)]]]] ∧
+  (type_to_AST (Tapp tys tycon) =
+    case tycon of
+        TC_fn => (case tys of
+                      [a;b] =>
+                      ND nType [
+                        ND nPType [
+                          ND nDType [
+                            ND nTbase [LF LparT; type_to_AST a; LF RparT]
+                          ]
+                        ];
+                        LF ArrowT;
+                        ND nType [
+                          ND nPType [
+                            ND nDType [
+                              ND nTbase [LF LparT; type_to_AST b; LF RparT]
+                            ]
+                          ]
+                        ]
+                      ]
+                    | _ => ARB)
+      | TC_tup => ND nType [typel_to_AST_PType tys]
+      | TC_name id =>
+        (let
+           tyop = tyname_to_AST id
+         in
+           case tys of
+               [] => ND nType [ND nPType [ND nDType [ND nTbase [tyop]]]]
+             | [ty] =>
+               ND nType [
+                 ND nPType [
+                   ND nDType [
+                     ND nDType [ND nTbase [LF LparT; type_to_AST ty; LF RparT]];
+                     tyop
+                   ]
+                 ]
+               ]
+             | ty1::tyrest =>
+               ND nType [
+                 ND nPType [
+                   ND nDType [
+                     ND nTbase [
+                       LF LparT;
+                       ND nTypeList2 [
+                         type_to_AST ty1; LF CommaT;
+                         typel_to_AST tyrest
+                       ];
+                       LF RparT;
+                       tyop
+                     ]
+                   ]
+                 ]
+               ])
+      | _ => ARB) ∧
+  typel_to_AST [] = ARB ∧
+  typel_to_AST [ty] = ND nTypeList1 [type_to_AST ty] ∧
+  typel_to_AST (ty1::tyrest) = ND nTypeList1 [type_to_AST ty1; LF CommaT;
+                                              typel_to_AST tyrest] ∧
+  typel_to_AST_PType [] = ARB ∧
+  typel_to_AST_PType [ty] =
+    ND nPType [ND nDType [ND nTbase [LF LparT; type_to_AST ty; LF RparT]]] ∧
+  typel_to_AST_PType (ty::tys) =
+    ND nPType [ND nDType [ND nTbase [LF LparT; type_to_AST ty; LF RparT]];
+               LF StarT;
+               typel_to_AST_PType tys]
+’ (WF_REL_TAC
+     ‘measure (λs. case s of INL ty => t_size ty
+                           | INR (INL tyl) => t1_size tyl
+                           | INR (INR tyl) => t1_size tyl)’)
+
+val destTyvarPT_tyname_to_AST = Q.store_thm(
+  "destTyvarPT_tyname_to_AST",
+  ‘∀i. user_expressible_tyname i ⇒ destTyvarPT (tyname_to_AST i) = NONE’,
+  Cases >> simp[tyname_to_AST_def] >>
+  rename [‘Long _ j’] >> Cases_on ‘j’ >>
+  simp[tyname_to_AST_def]);
+
+val types_inverted = Q.store_thm(
+  "types_inverted",
+  ‘(∀ty.
+     user_expressible_type ty ⇒ ptree_Type nType (type_to_AST ty) = SOME ty) ∧
+   (∀tys.
+     EVERY user_expressible_type tys ∧ tys ≠ [] ⇒
+     ptree_TypeList1 (typel_to_AST tys) = SOME tys) ∧
+   (∀tys.
+     EVERY user_expressible_type tys ∧ tys ≠ [] ⇒
+     ptree_PType (typel_to_AST_PType tys) = SOME tys)’,
+  ho_match_mp_tac (theorem "type_to_AST_ind") >>
+  rpt conj_tac >> simp[]
+  >- simp[ptree_Type_def, type_to_AST_def, tuplify_def]
+  >- (rpt strip_tac >>
+      rename [‘Tapp args tycon’] >> Cases_on ‘tycon’ >>
+      fs[]
+      >- (simp[type_to_AST_def] >> Cases_on ‘args’ >> simp[]
+          >- simp[Ntimes ptree_Type_def 5, tuplify_def,
+                  destTyvarPT_tyname_to_AST, tyname_inverted] >>
+          fs[] >>
+          rename [‘tl = []’] >> Cases_on ‘tl’
+          >- simp[ptree_Type_def, tuplify_def,
+                  destTyvarPT_tyname_to_AST, tyname_inverted,
+                  tokcheck_def] >>
+          fs[] >>
+          simp[Ntimes ptree_Type_def 6, tokcheck_def] >>
+          simp[tyname_inverted] >> dsimp[tuplify_def] >>
+          first_x_assum irule >>
+          full_simp_tac (srw_ss() ++ ETA_ss) [])
+      >- (simp[type_to_AST_def] >> fs[] >>
+          simp[ptree_Type_def, tokcheck_def, tuplify_def, astTheory.Tfn_def])
+      >- (rename [‘Tapp args TC_tup’] >>
+          simp[type_to_AST_def, Ntimes ptree_Type_def 1] >>
+          ‘args ≠ []’ by (strip_tac >> fs[]) >> fs[] >>
+          ‘∃x y xs. args = x::y::xs’
+            by (Cases_on ‘args’ >> fs[] >> rename [‘2 ≤ SUC (LENGTH rest)’] >>
+                Cases_on ‘rest’ >> fs[]) >>
+          simp[tuplify_def]))
+  >- (simp[Once ptree_Type_def] >> simp[type_to_AST_def])
+  >- (simp[type_to_AST_def] >> rpt strip_tac >> fs[] >>
+      simp[ptree_Type_def, tokcheck_def])
+  >- (simp[type_to_AST_def] >> simp[ptree_Type_def, tokcheck_def])
+  >- (simp[type_to_AST_def] >> rpt strip_tac >>
+      simp[Ntimes ptree_Type_def 6, tokcheck_def]));
+
 val ptree_head_TOK = Q.store_thm(
   "ptree_head_TOK",
   `(ptree_head pt = TOK sym ⇔ ?l. pt = Lf (TOK sym,l)) ∧
@@ -34,14 +201,14 @@ val TyOp_OK = Q.store_thm(
   "TyOp_OK",
   `valid_ptree cmlG pt ∧ ptree_head pt = NT (mkNT nTyOp) ∧
     MAP TK toks = ptree_fringe pt ⇒
-    ∃tyop. ptree_Tyop pt = SOME tyop`,
+    ∃tyop. ptree_Tyop pt = SOME tyop ∧ user_expressible_tyname tyop`,
   start >> simp[ptree_Tyop_def] >>
   asm_match `valid_ptree cmlG pt'` >>
   `destLf pt' = NONE`
     by (Cases_on `pt'` >> fs[MAP_EQ_CONS] >> rename [`Lf tokloc`] >>
         Cases_on `tokloc` >>
         rveq >> fs[] >> rveq >> fs[]) >>
-  simp[] >> metis_tac [UQTyOp_OK]);
+  dsimp[] >> metis_tac [UQTyOp_OK]);
 
 val TyvarN_OK = Q.store_thm(
   "TyvarN_OK",
@@ -79,7 +246,9 @@ val TypeName_OK = Q.store_thm(
 
 val tuplify_OK = Q.store_thm(
   "tuplify_OK",
-  `tl <> [] ⇒ ∃t. tuplify tl = SOME t`,
+  `tl <> [] ⇒
+   ∃t. tuplify tl = SOME t ∧
+       (EVERY user_expressible_type tl ⇒ user_expressible_type t)`,
   strip_tac >>
   `∃h tl0. tl = h::tl0` by (Cases_on `tl` >> fs[]) >>
   Cases_on `tl0` >> simp[tuplify_def]);
@@ -90,13 +259,14 @@ val Type_OK0 = Q.store_thm(
     (N ∈ {nType; nDType; nTbase} ∧
      ptree_head pt = NT (mkNT N)
        ⇒
-     ∃t. ptree_Type N pt = SOME t) ∧
+     ∃t. ptree_Type N pt = SOME t ∧ user_expressible_type t) ∧
     (ptree_head pt = NT (mkNT nPType) ⇒
-     ∃tl. ptree_PType pt = SOME tl ∧ tl <> []) ∧
+     ∃tl. ptree_PType pt = SOME tl ∧ tl <> [] ∧
+          EVERY user_expressible_type tl) ∧
     (ptree_head pt = NT (mkNT nTypeList1) ⇒
-     ∃tl. ptree_TypeList1 pt = SOME tl) ∧
+     ∃tl. ptree_TypeList1 pt = SOME tl ∧ EVERY user_expressible_type tl) ∧
     (ptree_head pt = NT (mkNT nTypeList2) ⇒
-     ∃tl. ptree_Typelist2 pt = SOME tl)`,
+     ∃tl. ptree_Typelist2 pt = SOME tl ∧ EVERY user_expressible_type tl)`,
   map_every qid_spec_tac [`N`, `toks`, `pt`] >>
   ho_match_mp_tac grammarTheory.ptree_ind >>
   conj_tac >> simp[Once FORALL_PROD] >>
@@ -106,21 +276,21 @@ val Type_OK0 = Q.store_thm(
   simp[Once ptree_Type_def] >>
   fs[DISJ_IMP_THM, FORALL_AND_THM, tokcheck_def]
   >- metis_tac[tuplify_OK]
-  >- metis_tac[tuplify_OK]
-  >- metis_tac[TyOp_OK]
+  >- (dsimp[astTheory.Tfn_def] >> metis_tac[tuplify_OK])
+  >- (dsimp[] >> metis_tac[TyOp_OK])
   >- metis_tac[]
   >- (rename1 `ptree_head pt'` >>
       `destTyvarPT pt' = NONE`
         by (Cases_on `pt'` >> fs[] >> rename[`Lf p`] >> Cases_on `p` >>
             fs[] >> fs[]) >>
-      simp[] >> metis_tac[TyOp_OK])
-  >- metis_tac [TyOp_OK]
+      dsimp[] >> metis_tac[TyOp_OK])
+  >- (dsimp[] >> metis_tac [TyOp_OK])
   >- metis_tac[]
   >- (dsimp[] >> metis_tac[])
   >- (dsimp[] >> metis_tac[])
-  >- metis_tac[]
-  >- metis_tac[]
-  >- metis_tac[])
+  >- (dsimp[] >> metis_tac[])
+  >- (dsimp[] >> metis_tac[])
+  >- (dsimp[] >> metis_tac[]));
 
 fun okify c q th =
     th |> UNDISCH |> c |> Q.INST [`N` |-> q]
